coq/proof/SoundForgetMemory.v
@@ -31,7 +31,7 @@ Set Implicit Arguments.
 
 Inductive mem_change : Type :=
 | mem_change_alloc
-    (def_var:id) (b:mblock) (ty:typ) (s:sz) (gn:GenericValue) (a:align)
+    (def_var:id) (ty:typ) (s:sz) (gn:GenericValue) (a:align)
 | mem_change_store
     (ptr:GenericValue) (ty:typ) (gv:GenericValue) (a:align)
 | mem_change_free
@@ -42,15 +42,15 @@ Inductive mem_change : Type :=
 Inductive mem_change_inject (conf_src conf_tgt:Config) invmem: mem_change -> mem_change -> Prop :=
 | mem_change_inject_alloc_alloc
     gsz gn0 gn1 a
-    b_src b_tgt ty dv
+    ty dv
     (N_INJECT: genericvalues_inject.gv_inject invmem.(InvMem.Rel.inject) gn0 gn1)
-  : mem_change_inject conf_src conf_tgt invmem (mem_change_alloc dv b_src ty gsz gn0 a) (mem_change_alloc dv b_tgt ty gsz gn1 a)
+  : mem_change_inject conf_src conf_tgt invmem (mem_change_alloc dv ty gsz gn0 a) (mem_change_alloc dv ty gsz gn1 a)
 | mem_change_inject_alloc_none
-    gsz gn a b ty dv
-  : mem_change_inject conf_src conf_tgt invmem (mem_change_alloc dv b ty gsz gn a) mem_change_none
+    gsz gn a ty dv
+  : mem_change_inject conf_src conf_tgt invmem (mem_change_alloc dv ty gsz gn a) mem_change_none
 | mem_change_inject_none_alloc
-    gsz gn a b ty dv
-  : mem_change_inject conf_src conf_tgt invmem mem_change_none (mem_change_alloc dv b ty gsz gn a)
+    gsz gn a ty dv
+  : mem_change_inject conf_src conf_tgt invmem mem_change_none (mem_change_alloc dv ty gsz gn a)
 | mem_change_inject_store_store
     ptr0 ptr1 gv0 gv1 ty a
     (PTR_INJECT: genericvalues_inject.gv_inject invmem.(InvMem.Rel.inject) ptr0 ptr1)
@@ -69,31 +69,66 @@ Inductive mem_change_inject (conf_src conf_tgt:Config) invmem: mem_change -> mem
     : mem_change_inject conf_src conf_tgt invmem mem_change_none mem_change_none
 .
 
-Inductive states_mem_change (conf:Config) (st0 st1:State): mem_change -> Prop :=
+Inductive states_mem_change conf mem0 mem1: mem_change -> Prop :=
 | states_mem_change_alloc
-    mb ty bsz gn a dv
-    (MALLOC: Some (st1.(Mem), mb) = malloc conf.(CurTargetData) st0.(Mem) bsz gn a)
-    (UNIQUE: InvState.Unary.sem_unique conf st0 dv)
-    (DEF_VAR: lookupAL _ st1.(EC).(Locals) dv = Some (blk2GV conf.(CurTargetData) mb))
-  : states_mem_change conf st0 st1 (mem_change_alloc dv mb ty bsz gn a)
+    ty bsz gn a dv mb
+    (MALLOC: Some (mem1, mb) = malloc conf.(CurTargetData) mem0 bsz gn a)
+  : states_mem_change conf mem0 mem1 (mem_change_alloc dv ty bsz gn a)
 | states_mem_change_store
     ptr ty gv a
-    (STORE: Some st1.(Mem) = mstore conf.(CurTargetData) st0.(Mem) ptr ty gv a)
-  : states_mem_change conf st0 st1 (mem_change_store ptr ty gv a)
+    (STORE: Some mem1 = mstore conf.(CurTargetData) mem0 ptr ty gv a)
+  : states_mem_change conf mem0 mem1 (mem_change_store ptr ty gv a)
 | states_mem_change_free
     ptr
-    (FREE: Some st1.(Mem) = free conf.(CurTargetData) st0.(Mem) ptr)
-  : states_mem_change conf st0 st1 (mem_change_free ptr)
+    (FREE: Some mem1 = free conf.(CurTargetData) mem0 ptr)
+  : states_mem_change conf mem0 mem1 (mem_change_free ptr)
 | states_mem_change_none
-    (MEM_EQ: st0.(Mem) = st1.(Mem))
-  : states_mem_change conf st0 st1 mem_change_none
+    (MEM_EQ: mem0 = mem1)
+  : states_mem_change conf mem0 mem1 mem_change_none
 .
 
-Inductive state_equiv_except_mem (conf:Config) (st0 st1:State) (mem_chng:mem_change) :=
-| state_equiv_except_mem_intro
-    (LOCALS_EQ: st0.(EC).(Locals) = st1.(EC).(Locals))
-    (STATES_MEM_CHANGE: states_mem_change conf st0 st1 mem_chng)
-.
+(* Relation between mem_change and cmd *)
+
+Definition mem_change_of_cmd conf cmd lc: option mem_change :=
+  match cmd with
+  | insn_alloca x ty v a =>
+    match getTypeAllocSize conf.(CurTargetData) ty,
+          getOperandValue conf.(CurTargetData) v lc conf.(Globals) with
+      | Some tsz, Some gn => Some (mem_change_alloc x ty tsz gn a)
+      | _, _ => None
+    end
+  | insn_store _ ty v_val v_ptr a =>
+    match getOperandValue conf.(CurTargetData) v_val lc conf.(Globals),
+          getOperandValue conf.(CurTargetData) v_ptr lc conf.(Globals) with
+    | Some gv_val, Some gv_ptr => Some (mem_change_store gv_ptr ty gv_val a)
+    | _, _ => None
+    end
+  | insn_free x _ v_ptr =>
+    match getOperandValue conf.(CurTargetData) v_ptr lc conf.(Globals) with
+    | Some gv_ptr => Some (mem_change_free gv_ptr)
+    | _ => None
+    end
+  | _ => Some mem_change_none
+  end.
+
+Definition mem_change_cmd_after conf st mc cmd inv0: Prop :=
+  match cmd with
+  | insn_alloca dv ty v a =>
+    exists tsz gn,
+    <<TYPE: getTypeAllocSize conf.(CurTargetData) ty = Some tsz>> /\
+    <<FORGET: inv_unary_forgot inv0 (AtomSetImpl_from_list [dv])>> /\
+    <<MEM_CH: mc = mem_change_alloc dv ty tsz gn a>>
+  | insn_store _ ty v_val v_ptr a =>
+    exists gv_val gv_ptr,
+    <<VAL: getOperandValue conf.(CurTargetData) v_val st.(EC).(Locals) conf.(Globals) = Some gv_val>> /\
+    <<PTR: getOperandValue conf.(CurTargetData) v_ptr st.(EC).(Locals) conf.(Globals) = Some gv_ptr>> /\
+    <<MEM_CH: mc = mem_change_store gv_ptr ty gv_val a>>
+  | insn_free dv _ v_ptr =>
+    exists gv_ptr,
+    <<PTR: getOperandValue conf.(CurTargetData) v_ptr st.(EC).(Locals) conf.(Globals) = Some gv_ptr>> /\
+    <<MEM_CH: mc = mem_change_free gv_ptr>>
+  | _ => mc = mem_change_none
+  end.
 
 (* proof for private_parent *)
 
@@ -183,62 +218,6 @@ Proof.
   - exploit PRIVATE_PARENT; eauto. i. des.
     hexploit gv_inject_ptr_public_tgt; try apply PTR; eauto.
 Qed.
-
-(* Difference btw rel and rel_after: changing locals & forget *)
-
-Definition mem_change_cmd conf st mc cmd: Prop :=
-  match cmd with
-  | insn_alloca dv ty v a =>
-    exists mb tsz gn,
-    <<TYPE: getTypeAllocSize conf.(CurTargetData) ty = Some tsz>> /\
-    <<VAL: getOperandValue conf.(CurTargetData) v st.(EC).(Locals) conf.(Globals) = Some gn>> /\
-    <<MEM_CH: mc = mem_change_alloc dv mb ty tsz gn a>>
-  | insn_malloc dv ty v a =>
-    exists mb tsz gn,
-    <<TYPE: getTypeAllocSize conf.(CurTargetData) ty = Some tsz>> /\
-    <<VAL: getOperandValue conf.(CurTargetData) v st.(EC).(Locals) conf.(Globals) = Some gn>> /\
-    <<MEM_CH: mc = mem_change_alloc dv mb ty tsz gn a>>
-  | insn_store _ ty v_val v_ptr a =>
-    exists gv_val gv_ptr,
-    <<VAL: getOperandValue conf.(CurTargetData) v_val st.(EC).(Locals) conf.(Globals) = Some gv_val>> /\
-    <<PTR: getOperandValue conf.(CurTargetData) v_ptr st.(EC).(Locals) conf.(Globals) = Some gv_ptr>> /\
-    <<MEM_CH: mc = mem_change_store gv_ptr ty gv_val a>>
-  | insn_free dv _ v_ptr =>
-    exists gv_ptr,
-    <<PTR: getOperandValue conf.(CurTargetData) v_ptr st.(EC).(Locals) conf.(Globals) = Some gv_ptr>> /\
-    <<MEM_CH: mc = mem_change_free gv_ptr>>
-  | _ => mc = mem_change_none
-  end.
-
-Definition mem_change_cmd_after conf st mc cmd inv0: Prop :=
-  match cmd with
-  | insn_alloca dv ty v a =>
-    exists mb tsz gn,
-    <<TYPE: getTypeAllocSize conf.(CurTargetData) ty = Some tsz>> /\
-    (* <<VAL: getOperandValue conf.(CurTargetData) v st.(EC).(Locals) conf.(Globals) = Some gn>> /\ *)
-    <<FORGET: inv_unary_forgot inv0 (AtomSetImpl.singleton dv)>> /\
-    <<MEM_CH: mc = mem_change_alloc dv mb ty tsz gn a>>
-  | insn_malloc dv ty v a =>
-    exists mb tsz gn,
-    <<TYPE: getTypeAllocSize conf.(CurTargetData) ty = Some tsz>> /\
-    (* <<VAL: getOperandValue conf.(CurTargetData) v st.(EC).(Locals) conf.(Globals) = Some gn>> /\ *)
-    <<FORGET: inv_unary_forgot inv0 (AtomSetImpl.singleton dv)>> /\
-    <<MEM_CH: mc = mem_change_alloc dv mb ty tsz gn a>>
-  | insn_store _ ty v_val v_ptr a =>
-    exists gv_val gv_ptr,
-    <<VAL: getOperandValue conf.(CurTargetData) v_val st.(EC).(Locals) conf.(Globals) = Some gv_val>> /\
-    <<PTR: getOperandValue conf.(CurTargetData) v_ptr st.(EC).(Locals) conf.(Globals) = Some gv_ptr>> /\
-    <<MEM_CH: mc = mem_change_store gv_ptr ty gv_val a>>
-  | insn_free dv _ v_ptr =>
-    exists gv_ptr,
-    <<PTR: getOperandValue conf.(CurTargetData) v_ptr st.(EC).(Locals) conf.(Globals) = Some gv_ptr>> /\
-    <<MEM_CH: mc = mem_change_free gv_ptr>>
-  | _ => mc = mem_change_none
-  end.
-
-Definition unique_preserved_mem conf st inv: Prop :=
-  forall u (MEM: AtomSetImpl.mem u inv.(Invariant.unique) = true),
-    InvState.Unary.sem_unique conf st u.
 
 (* Subset *)
 
@@ -392,293 +371,557 @@ Qed.
 
 (* soundness proof *)
 
-Lemma forget_memory_unary_sound1
-      conf st0 invst0 invmem0 inv0
-      cmd st1 public gmax mem_change def_memory
+Definition unique_preserved_mem conf st inv: Prop :=
+  forall u (MEM: AtomSetImpl.mem u inv.(Invariant.unique) = true),
+    InvState.Unary.sem_unique conf st u.
+
+Definition alloc_inject conf_src conf_tgt st1_src st1_tgt cmd_src cmd_tgt invmem1 : Prop :=
+  forall x ty v_src v_tgt a
+         (ALLOCA_SRC: cmd_src = insn_alloca x ty v_src a)
+         (ALLOCA_TGT: cmd_tgt = insn_alloca x ty v_tgt a),
+    exists b_src b_tgt gptr_src gptr_tgt,
+      lookupAL _ st1_src.(EC).(Locals) x = Some gptr_src /\
+      lookupAL _ st1_tgt.(EC).(Locals) x = Some gptr_tgt /\
+      GV2ptr conf_src.(CurTargetData) conf_src.(CurTargetData).(getPointerSize) gptr_src =
+      Some (Values.Vptr b_src (Integers.Int.zero 31)) /\
+      GV2ptr conf_tgt.(CurTargetData) conf_tgt.(CurTargetData).(getPointerSize) gptr_tgt =
+      Some (Values.Vptr b_tgt (Integers.Int.zero 31)) /\
+      invmem1.(InvMem.Rel.inject) b_src = Some (b_tgt, 0).
+
+Lemma step_mem_change
+      st0 st1 invst0 invmem0 inv0 inv1
+      cmd cmds
+      conf evt
       (STATE: InvState.Unary.sem conf st0 invst0 invmem0 inv0)
-      (DEF_MEM: Cmd.get_def_memory cmd = Some def_memory)
-      (MEM: InvMem.Unary.sem conf gmax public st0.(Mem) invmem0)
-      (MEM_EQUIV: state_equiv_except_mem conf st0 st1 mem_change)
-      (MEM_CHANGE: mem_change_cmd_after conf st0 mem_change cmd inv0)
-      (NO_PRIVATE_PARENT: mem_change_no_private_parent conf mem_change invmem0.(InvMem.Unary.private_parent))
-      (UNIQUE_PRSV: unique_preserved_mem conf st1 inv0)
-  : <<STATE_UNARY: InvState.Unary.sem conf st1 invst0 invmem0 (ForgetMemory.unary def_memory inv0)>> /\
-                   <<MEM_UNARY: InvMem.Unary.sem conf gmax public st1.(Mem) invmem0>>.
+      (CMD: st0.(EC).(CurCmds) = cmd::cmds)
+      (NONCALL: Instruction.isCallInst cmd = false)
+      (STEP: sInsn conf st0 st1 evt)
+      (FORGET_DEFS: inv_unary_forgot inv1 (AtomSetImpl_from_list (option_to_list (Cmd.get_def cmd))))
+  : exists mc,
+    <<MC_SOME: mem_change_of_cmd conf cmd st0.(EC).(Locals) = Some mc>> /\
+    <<MC_AFTER: mem_change_cmd_after conf (mkState st1.(EC) st1.(ECS) st0.(Mem)) mc cmd inv1>> /\
+    <<STATE_EQUIV: states_mem_change conf st0.(Mem) st1.(Mem) mc>>.
 Proof.
-  destruct mem_change;
-    try by (destruct cmd; ss; des; congruence).
-  - splits.
-    admit.
-    admit.
-    
-    
-    (* + econs. *)
-    (*   { ii. ss. unfold ForgetMemory.unary in *. *)
-    (*     exploit forget_memory_def_sep_mem; eauto. i. *)
-    (*     exploit sem_expr_equiv_except_mem; eauto. *)
-    (*     { instantiate (1:= (fst x)). *)
-    (*       des; try by left; eauto. *)
-    (*       right. unfold ForgetMemory.is_noalias_ExprPair in *. des_bool. des. ss. *)
-    (*     } *)
-    (*     exploit sem_expr_equiv_except_mem; eauto. *)
-    (*     { instantiate (1:= (snd x)). *)
-    (*       des; try by left; eauto. *)
-    (*       right. unfold ForgetMemory.is_noalias_ExprPair in *. des_bool. des. ss. *)
-    (*     } *)
-    (*     i. *)
-    (*     inv STATE. *)
-    (*     exploit LESSDEF. *)
-    (*     { des_ifs; eauto. *)
-    (*       ss. eapply ExprPairSetFacts.filter_iff in H; eauto; try by solve_compat_bool. inv H; eauto. *)
-    (*     } *)
-    (*     { rewrite x0. eauto. } *)
-    (*     i. rewrite <- x2. eauto. *)
-    (*   } *)
-    (*   { admit. (* alias *) } *)
-    (*   { admit. } *)
-    (*   { admit. } *)
-    (* + inv MEM_EQUIV. *)
-    (*   inv MEM_CHANGE_EQUIV. *)
-    (*   inv MEM. *)
-    (*   econs; eauto. *)
-    (*   { i. exploit PRIVATE; eauto. i. des. *)
-    (*     split; eauto. *)
-    (*     admit. (* nextblock preserved after mstore *) } *)
-    (*   { i. exploit PRIVATE_PARENT; eauto. i. des. *)
-    (*     split; eauto. *)
-    (*     admit. (* same *) } *)
-    (*   { unfold mem_change_no_private_parent in *. *)
-    (*     i. exploit MEM_PARENT; eauto. *)
-    (*     i. rewrite x. *)
-    (*     (* STORE: (Mem st1) = mstore (Mem st0) ptr .. *) *)
-    (*     (* mstore says GV2ptr ptr = Some Vptr .. *) *)
-    (*     (* NO_PRIVATE_PARENT tells us ~In b_ptr (private_parent) *) *)
-    (*     (* since b is In private_parent, mload_aux ?mem b should be preserved *) *)
-    (*     admit. *)
-    (*   } *)
-  
-  - admit. (* free case - almost same as above *)
+  inv STEP; ss;
+    try by inv CMD;
+    esplits; ss; econs; eauto.
+  - admit. (* not malloc *)
+  - inv CMD.
+    esplits; ss.
+    + des_ifs.
+    + esplits; eauto.
+    + econs; eauto.
+  - inv CMD.
+    esplits; ss.
+    + des_ifs.
+    + esplits; eauto.
+    + econs; eauto.
+  - inv CMD.
+    esplits; ss.
+    + des_ifs.
+    + esplits; eauto.
+    + econs; eauto.
 Admitted.
 
-Lemma forget_memory_unary_sound2
-      conf st0 st1 mem_change
-      cmd invst0 invmem0 inv0 gmax public
-      (STATE: InvState.Unary.sem conf st0 invst0 invmem0 inv0)
-      (DEF_MEM: Cmd.get_def_memory cmd = None)
-      (MEM: InvMem.Unary.sem conf gmax public st0.(Mem) invmem0)
-      (MEM_EQUIV : state_equiv_except_mem conf st0 st1 mem_change)
-      (MEM_CHANGE : mem_change_cmd_after conf st0 mem_change cmd inv0)
-      (NO_PRIVATE_PARENT: mem_change_no_private_parent conf mem_change invmem0.(InvMem.Unary.private_parent))
-      (UNIQUE_PRSV: unique_preserved_mem conf st1 inv0)
-  : <<STATE_UNARY: InvState.Unary.sem conf st1 invst0 invmem0 inv0>> /\
-    <<MEM_UNARY: InvMem.Unary.sem conf gmax public st1.(Mem) invmem0>>.
+Lemma malloc_nextblock
+      TD mem mem' sz gn a mb
+      (MALLOC: malloc TD mem sz gn a = Some (mem', mb))
+  : <<ALLOC_BLOCK: mb = mem.(Memory.Mem.nextblock)>> /\
+    <<NEXT_BLOCK: mem'.(Memory.Mem.nextblock) = Pos.succ mem.(Memory.Mem.nextblock)>>
+.
 Proof.
-  destruct mem_change.
-  - destruct cmd; ss.
-    + admit. (* TODO: doing here *)
-    + admit. (* exactly same as above *)
-  - destruct cmd; ss; des; congruence.
-  - destruct cmd; ss; des; congruence.
-  - inv MEM_EQUIV. inv STATES_MEM_CHANGE.
-    rewrite <- MEM_EQ.
-    esplits; eauto.
-    eapply unary_sem_eq_locals_mem; try (symmetry in LOCALS_EQ; exact LOCALS_EQ); eauto.
+  unfold malloc in *.
+  des_ifs.
+Qed.
+
+Lemma inject_mem_change
+      conf_src cmd_src mc_src st0_src
+      conf_tgt cmd_tgt mc_tgt st0_tgt
+      inv0 invmem0 invst0
+      (STATE : InvState.Rel.sem conf_src conf_tgt st0_src st0_tgt invst0 invmem0 inv0)
+      (INJECT_EVENT : postcond_cmd_inject_event cmd_src cmd_tgt inv0)
+      (MC_SRC : mem_change_of_cmd conf_src cmd_src st0_src.(EC).(Locals) = Some mc_src)
+      (MC_TGT : mem_change_of_cmd conf_tgt cmd_tgt st0_tgt.(EC).(Locals) = Some mc_tgt)
+  : mem_change_inject conf_src conf_tgt invmem0 mc_src mc_tgt.
+Proof.
 Admitted.
 
-Lemma forget_memory_maydiff_preserved
-      conf_src st0_src st1_src mem_change_src def_mem_src
-      conf_tgt st0_tgt st1_tgt mem_change_tgt def_mem_tgt
-      invst0 invmem0 inv0
-      (MEM_EQUIV_SRC : state_equiv_except_mem conf_src st0_src st1_src mem_change_src)
-      (MEM_EQUIV_TGT : state_equiv_except_mem conf_tgt st0_tgt st1_tgt mem_change_tgt)
-      (MAYDIFF : forall id : Tag.t * id,
-          IdTSet.mem id (Invariant.maydiff inv0) = false ->
-          InvState.Rel.sem_inject st0_src st0_tgt invst0 (InvMem.Rel.inject invmem0) id)
-  : <<RES: forall id : Tag.t * id,
-      IdTSet.mem id (Invariant.maydiff (ForgetMemory.t def_mem_src def_mem_tgt inv0)) = false ->
-      InvState.Rel.sem_inject st1_src st1_tgt invst0 (InvMem.Rel.inject invmem0) id>>.
+Lemma inject_invmem
+      conf_src st0_src st1_src cmd_src cmds_src evt_src
+      conf_tgt st0_tgt st1_tgt cmd_tgt cmds_tgt evt_tgt
+      invst0 invmem0 inv0 inv1
+      (STATE : InvState.Rel.sem conf_src conf_tgt st0_src st0_tgt invst0 invmem0 inv0)
+      (MEM : InvMem.Rel.sem conf_src conf_tgt (Mem st0_src) (Mem st0_tgt) invmem0)
+      (CMD_SRC : CurCmds (EC st0_src) = cmd_src :: cmds_src)
+      (CMD_TGT : CurCmds (EC st0_tgt) = cmd_tgt :: cmds_tgt)
+      (NONCALL_SRC: Instruction.isCallInst cmd_src = false)
+      (NONCALL_TGT: Instruction.isCallInst cmd_tgt = false)
+      (STEP_SRC : sInsn conf_src st0_src st1_src evt_src)
+      (STEP_TGT : sInsn conf_tgt st0_tgt st1_tgt evt_tgt)
+      (INJECT_EVENT : postcond_cmd_inject_event cmd_src cmd_tgt inv0)
+      (FORGOT_SRC: inv_unary_forgot inv1.(Invariant.src) (AtomSetImpl_from_list (Cmd.get_def cmd_src)))
+      (FORGOT_TGT: inv_unary_forgot inv1.(Invariant.tgt) (AtomSetImpl_from_list (Cmd.get_def cmd_tgt)))
+  : exists invmem1,
+    <<ALLOC_INJECT: alloc_inject conf_src conf_tgt st1_src st1_tgt cmd_src cmd_tgt invmem1>> /\
+    <<MEM: InvMem.Rel.sem conf_src conf_tgt (Mem st1_src) (Mem st1_tgt) invmem1 >> /\
+    <<MEMLE: InvMem.Rel.le invmem0 invmem1 >>.
 Proof.
-  ii.
-  assert (DROP_FORGET_MEMORY:IdTSet.mem id0 (Invariant.maydiff inv0) = false).
-  { destruct def_mem_src; destruct def_mem_tgt; ss. }
-  exploit MAYDIFF; eauto.
-  { inv MEM_EQUIV_SRC.
-    unfold InvState.Unary.sem_idT in *.
-    destruct id0 as [[] x]; eauto.
-    ss. rewrite LOCALS_EQ. eauto.
-  }
-  i. des.
-  esplits; eauto.
-  inv MEM_EQUIV_TGT.
-  unfold InvState.Unary.sem_idT in *.
-  destruct id0 as [[] x]; eauto.
-  ss. rewrite <- LOCALS_EQ. eauto.
-Qed.
+  (* TODO: mc ~ mc0 *)
+Admitted.
 
-Lemma some_injective A (a b:A):
-  Some a = Some b -> a = b.
+Lemma forget_memory_equiv_except_mem
+      conf_src mem0_src st1_src mc_src cmd_src lc_src
+      conf_tgt mem0_tgt st1_tgt mc_tgt cmd_tgt lc_tgt
+      inv1 invst0 invmem0
+      (STATE_FORGET : InvState.Rel.sem conf_src conf_tgt
+                                       (mkState st1_src.(EC) st1_src.(ECS) mem0_src)
+                                       (mkState st1_tgt.(EC) st1_tgt.(ECS) mem0_tgt)
+                                       invst0 invmem0 inv1)
+      (MC_SOME_SRC : mem_change_of_cmd conf_src cmd_src lc_src = Some mc_src)
+      (MC_SOME_TGT : mem_change_of_cmd conf_tgt cmd_tgt lc_tgt = Some mc_tgt)
+      (STATE_EQUIV_SRC : states_mem_change conf_src mem0_src st1_src.(Mem) mc_src)
+      (STATE_EQUIV_TGT : states_mem_change conf_tgt mem0_tgt st1_tgt.(Mem) mc_tgt)
+  : InvState.Rel.sem conf_src conf_tgt st1_src st1_tgt invst0 invmem0
+                     (ForgetMemory.t (Cmd.get_def_memory cmd_src) (Cmd.get_def_memory cmd_tgt) inv1).
 Proof.
-  congruence.
-Qed.
-
-Lemma mem_inject_change
-      conf_src st0_src st1_src mem_change_src
-      conf_tgt st0_tgt st1_tgt mem_change_tgt
-      invmem0
-      (MEM_CHANGE_EQUIV_SRC : states_mem_change conf_src st0_src st1_src mem_change_src)
-      (MEM_CHANGE_EQUIV_TGT : states_mem_change conf_tgt st0_tgt st1_tgt mem_change_tgt)
-      (MEM_CHANGE_INJECT : mem_change_inject conf_src conf_tgt invmem0 mem_change_src mem_change_tgt)
-      (INJECT : Memory.Mem.inject invmem0.(InvMem.Rel.inject) st0_src.(Mem) st0_tgt.(Mem))
-  : Memory.Mem.inject invmem0.(InvMem.Rel.inject) st1_src.(Mem) st1_tgt.(Mem).
-Proof.
-  inv MEM_CHANGE_INJECT.
-  - inv INJECT. inv MEM_CHANGE_EQUIV_SRC. inv MEM_CHANGE_EQUIV_TGT.
-    unfold malloc in *.
-    apply some_injective in MALLOC.
-    apply some_injective in MALLOC0.
-    econs.
-    + eapply Memory.Mem.alloc_right_inj; eauto.
-      eapply Memory.Mem.alloc_left_unmapped_inj; eauto.
-      apply mi_freeblocks.
-      eapply Memory.Mem.fresh_block_alloc; eauto.
-    + i. apply mi_freeblocks. ii.
-      exploit Memory.Mem.valid_block_alloc; try (symmetry; exact MALLOC); eauto.
-    + ii. exploit mi_mappedblocks; eauto. i.
-      eapply Memory.Mem.valid_block_alloc; eauto.
-    + ii. exploit mi_no_overlap; eauto.
-      * eapply Memory.Mem.perm_alloc_4; try (symmetry; exact MALLOC); eauto.
-        ii. subst.
-        hexploit Memory.Mem.fresh_block_alloc; try (symmetry; exact MALLOC); eauto. i.
-        exploit mi_freeblocks; eauto. i. clarify.
-      * eapply Memory.Mem.perm_alloc_4; try (symmetry; exact MALLOC); eauto.
-        ii. subst.
-        hexploit Memory.Mem.fresh_block_alloc; try (symmetry; exact MALLOC); eauto. i.
-        exploit mi_freeblocks; eauto. i. clarify.
-    + ii. exploit mi_representable; eauto. des.
-      * left.
-        eapply Memory.Mem.perm_alloc_4; try (symmetry; exact MALLOC); eauto.
-        ii. subst.
-        hexploit Memory.Mem.fresh_block_alloc; try (symmetry; exact MALLOC); eauto. i.
-        exploit mi_freeblocks; eauto. i. clarify.
-      * right.
-        eapply Memory.Mem.perm_alloc_4; try (symmetry; exact MALLOC); eauto.
-        ii. subst.
-        hexploit Memory.Mem.fresh_block_alloc; try (symmetry; exact MALLOC); eauto. i.
-        exploit mi_freeblocks; eauto. i. clarify.
-  - inv INJECT. inv MEM_CHANGE_EQUIV_SRC. inv MEM_CHANGE_EQUIV_TGT.
-    rewrite <- MEM_EQ; clear MEM_EQ.
-    unfold malloc in *.
-    apply some_injective in MALLOC.
-    econs.
-    + eapply Memory.Mem.alloc_left_unmapped_inj; eauto.
-      apply mi_freeblocks.
-      eapply Memory.Mem.fresh_block_alloc; eauto.
-    + i. apply mi_freeblocks. ii.
-      exploit Memory.Mem.valid_block_alloc; try (symmetry; exact MALLOC); eauto.
-    + ii. exploit mi_mappedblocks; eauto.
-    + ii. exploit mi_no_overlap; eauto.
-      * eapply Memory.Mem.perm_alloc_4; try (symmetry; exact MALLOC); eauto.
-        ii. subst.
-        hexploit Memory.Mem.fresh_block_alloc; try (symmetry; exact MALLOC); eauto. i.
-        exploit mi_freeblocks; eauto. i. clarify.
-      * eapply Memory.Mem.perm_alloc_4; try (symmetry; exact MALLOC); eauto.
-        ii. subst.
-        hexploit Memory.Mem.fresh_block_alloc; try (symmetry; exact MALLOC); eauto. i.
-        exploit mi_freeblocks; eauto. i. clarify.
-    + ii. exploit mi_representable; eauto. des.
-      * left.
-        eapply Memory.Mem.perm_alloc_4; try (symmetry; exact MALLOC); eauto.
-        ii. subst.
-        hexploit Memory.Mem.fresh_block_alloc; try (symmetry; exact MALLOC); eauto. i.
-        exploit mi_freeblocks; eauto. i. clarify.
-      * right.
-        eapply Memory.Mem.perm_alloc_4; try (symmetry; exact MALLOC); eauto.
-        ii. subst.
-        hexploit Memory.Mem.fresh_block_alloc; try (symmetry; exact MALLOC); eauto. i.
-        exploit mi_freeblocks; eauto. i. clarify.
-  - inv INJECT. inv MEM_CHANGE_EQUIV_SRC. inv MEM_CHANGE_EQUIV_TGT.
-    rewrite <- MEM_EQ; clear MEM_EQ.
-    unfold malloc in *.
-    apply some_injective in MALLOC.
-    econs.
-    + eapply Memory.Mem.alloc_right_inj; eauto.
-    + i. apply mi_freeblocks. eauto.
-    + ii. exploit mi_mappedblocks; eauto. i.
-      eapply Memory.Mem.valid_block_alloc; eauto.
-    + ii. exploit mi_no_overlap; eauto.
-    + ii. exploit mi_representable; eauto.
-  - inv MEM_CHANGE_EQUIV_SRC. inv MEM_CHANGE_EQUIV_TGT.
-    unfold mstore in *. des_ifs.
-    (* exploit genericvalues_inject.mem_inj_mstore_aux; eauto. *)
-    
-    (* Memory.Mem.mem_inj *)
-    (*   memory_sim.MoreMem.mem_inj *)
-    admit. (* store - store *)
-  - inv MEM_CHANGE_EQUIV_SRC. inv MEM_CHANGE_EQUIV_TGT.
-    unfold mstore in *. des_ifs.
-    admit. (* store to private *)
-    
-  - inv MEM_CHANGE_EQUIV_SRC. inv MEM_CHANGE_EQUIV_TGT.
-    unfold free in *. des_ifs.
-    eapply Memory.Mem.free_left_inject; eauto.
-    eapply Memory.Mem.free_right_inject; eauto.
-    admit. (* free - free *)
-  - inv MEM_CHANGE_EQUIV_SRC. inv MEM_CHANGE_EQUIV_TGT.
-    eauto.
 Admitted.
 
 Lemma forget_memory_sound
-      m_src conf_src st0_src st1_src mem_change_src cmd_src
-      m_tgt conf_tgt st0_tgt st1_tgt mem_change_tgt cmd_tgt
-      invst0 invmem0 inv0
+      m_src conf_src st0_src st1_src cmd_src cmds_src evt_src
+      m_tgt conf_tgt st0_tgt st1_tgt cmd_tgt cmds_tgt evt_tgt
+      invst0 invmem0 inv0 inv1
       (CONF: InvState.valid_conf m_src m_tgt conf_src conf_tgt)
       (STATE: InvState.Rel.sem conf_src conf_tgt st0_src st0_tgt invst0 invmem0 inv0)
+      (CMD_SRC: st0_src.(EC).(CurCmds) = cmd_src::cmds_src)
+      (CMD_TGT: st0_tgt.(EC).(CurCmds) = cmd_tgt::cmds_tgt)
+      (NONCALL_SRC: Instruction.isCallInst cmd_src = false)
+      (NONCALL_TGT: Instruction.isCallInst cmd_tgt = false)
+      (STEP_SRC: sInsn conf_src st0_src st1_src evt_src)
+      (STEP_TGT: sInsn conf_tgt st0_tgt st1_tgt evt_tgt)
+      (INJECT_EVENT: postcond_cmd_inject_event cmd_src cmd_tgt inv0)
       (MEM: InvMem.Rel.sem conf_src conf_tgt st0_src.(Mem) st0_tgt.(Mem) invmem0)
-      (MEM_EQUIV_SRC: state_equiv_except_mem
-                        conf_src
-                        st0_src st1_src
-                        mem_change_src)
-      (MEM_EQUIV_TGT: state_equiv_except_mem
-                        conf_tgt
-                        st0_tgt st1_tgt
-                        mem_change_tgt)
-      (MEM_CHANGE_SRC: mem_change_cmd_after conf_src st0_src mem_change_src cmd_src inv0.(Invariant.src))
-      (MEM_CHANGE_TGT: mem_change_cmd_after conf_tgt st0_tgt mem_change_tgt cmd_tgt inv0.(Invariant.tgt))
-      (MEM_CHANGE_INJECT: mem_change_inject conf_src conf_tgt invmem0 mem_change_src mem_change_tgt)
-      (UNIQUE_PRSV_SRC: unique_preserved_mem conf_src st1_src inv0.(Invariant.src))
-      (UNIQUE_PRSV_TGT: unique_preserved_mem conf_tgt st1_tgt inv0.(Invariant.tgt))
-  : <<STATE: InvState.Rel.sem conf_src conf_tgt st1_src st1_tgt invst0 invmem0
-                              (ForgetMemory.t (Cmd.get_def_memory cmd_src) (Cmd.get_def_memory cmd_tgt) inv0) >> /\
-    <<MEM: InvMem.Rel.sem conf_src conf_tgt st1_src.(Mem) st1_tgt.(Mem) invmem0>>.
+      (FORGOT_SRC: inv_unary_forgot inv1.(Invariant.src)
+                                                (AtomSetImpl_from_list (option_to_list (Cmd.get_def cmd_src))))
+      (FORGOT_TGT: inv_unary_forgot inv1.(Invariant.tgt)
+                                                (AtomSetImpl_from_list (option_to_list (Cmd.get_def cmd_tgt))))
+      (STATE_FORGET: InvState.Rel.sem conf_src conf_tgt
+                                      (mkState st1_src.(EC) st1_src.(ECS) st0_src.(Mem))
+                                      (mkState st1_tgt.(EC) st1_tgt.(ECS) st0_tgt.(Mem))
+                                      invst0 invmem0 inv1)
+      (UNIQUE_PRSV_SRC: unique_preserved_mem conf_src st1_src inv1.(Invariant.src))
+      (UNIQUE_PRSV_TGT: unique_preserved_mem conf_tgt st1_tgt inv1.(Invariant.tgt))
+  :
+    exists invmem1,
+      <<ALLOC_INJECT: alloc_inject conf_src conf_tgt st1_src st1_tgt cmd_src cmd_tgt invmem1>> /\
+      <<STATE: InvState.Rel.sem conf_src conf_tgt st1_src st1_tgt invst0 invmem1
+                                (ForgetMemory.t (Cmd.get_def_memory cmd_src) (Cmd.get_def_memory cmd_tgt) inv1) >> /\
+      <<MEM: InvMem.Rel.sem conf_src conf_tgt st1_src.(Mem) st1_tgt.(Mem) invmem1>> /\
+      <<MEMLE: InvMem.Rel.le invmem0 invmem1>>.
 Proof.
-  exploit mem_change_inject_no_private_parent_src; eauto. intro NO_PRIVATE_PARENT_SRC.
-  exploit mem_change_inject_no_private_parent_tgt; eauto. intro NO_PRIVATE_PARENT_TGT.
-  inv STATE. inv MEM.
+  exploit step_mem_change.
+  { inv STATE. exact SRC. }
+  { eauto. }
+  { eauto. }
+  { eauto. }
+  { eauto. }
+  exploit step_mem_change.
+  { inv STATE. exact TGT. }
+  { eauto. }
+  { eauto. }
+  { eauto. }
+  { eauto. }
+  i. des.
 
-  destruct (Cmd.get_def_memory cmd_src) eqn:DEF_MEM_SRC;
-    destruct (Cmd.get_def_memory cmd_tgt) eqn:DEF_MEM_TGT.
-  - hexploit forget_memory_unary_sound1; try exact SRC; try exact DEF_MEM_SRC; eauto. i. des.
-    hexploit forget_memory_unary_sound1; try exact TGT; try exact DEF_MEM_TGT; eauto. i. des.
-    hexploit forget_memory_maydiff_preserved; try exact MAYDIFF; eauto. i. des.
-    inv MEM_EQUIV_SRC. inv MEM_EQUIV_TGT.
-    hexploit mem_inject_change; try exact MEM_CHANGE_INJECT; eauto. i.
-    esplits; econs; eauto.
-  - hexploit forget_memory_unary_sound1; try exact SRC; try exact DEF_MEM_SRC; eauto. i. des.
-    hexploit forget_memory_unary_sound2; try exact TGT; try exact DEF_MEM_TGT; eauto. i. des.
-    hexploit forget_memory_maydiff_preserved; try exact MAYDIFF; eauto. i. des.
-    inv MEM_EQUIV_SRC. inv MEM_EQUIV_TGT.
-    hexploit mem_inject_change; try exact MEM_CHANGE_INJECT; eauto. i.
-    esplits; econs; eauto.
-  - hexploit forget_memory_unary_sound2; try exact SRC; try exact DEF_MEM_SRC; eauto. i. des.
-    hexploit forget_memory_unary_sound1; try exact TGT; try exact DEF_MEM_TGT; eauto. i. des.
-    hexploit forget_memory_maydiff_preserved; try exact MAYDIFF; eauto. i. des.
-    inv MEM_EQUIV_SRC. inv MEM_EQUIV_TGT.
-    hexploit mem_inject_change; try exact MEM_CHANGE_INJECT; eauto. i.
-    esplits; econs; eauto.
-  - hexploit forget_memory_unary_sound2; try exact SRC; try exact DEF_MEM_SRC; eauto. i. des.
-    hexploit forget_memory_unary_sound2; try exact TGT; try exact DEF_MEM_TGT; eauto. i. des.
-    hexploit forget_memory_maydiff_preserved; try exact MAYDIFF; eauto. i. des.
-    inv MEM_EQUIV_SRC. inv MEM_EQUIV_TGT.
-    hexploit mem_inject_change; try exact MEM_CHANGE_INJECT; eauto. i.
-    esplits; econs; eauto.
-Qed.
+  exploit inject_invmem; try exact INJECT_EVENT; eauto.
+  i. des.
+  esplits; eauto.
+
+  eapply forget_memory_equiv_except_mem; eauto.
+  admit. (* InvState.Rel.mem monotone w.r.t. invmem1 *)
+Admitted.
+
+(* until here *)
+
+
+
+(* Lemma forget_memory_unary_sound_with_def_memory *)
+(*       conf st0 invst0 invmem0 inv0 *)
+(*       cmd st1 public gmax mem_change def_memory *)
+(*       (STATE: InvState.Unary.sem conf st0 invst0 invmem0 inv0) *)
+(*       (DEF_MEM: Cmd.get_def_memory cmd = Some def_memory) *)
+(*       (MEM: InvMem.Unary.sem conf gmax public st0.(Mem) invmem0) *)
+(*       (MEM_EQUIV: state_equiv_except_mem conf st0 st1 mem_change) *)
+(*       (MEM_CHANGE: mem_change_cmd_after conf st0 mem_change cmd inv0) *)
+(*       (NO_PRIVATE_PARENT: mem_change_no_private_parent conf mem_change invmem0.(InvMem.Unary.private_parent)) *)
+(*       (UNIQUE_PRSV: unique_preserved_mem conf st1 inv0) *)
+(*   : <<STATE_UNARY: InvState.Unary.sem conf st1 invst0 invmem0 (ForgetMemory.unary def_memory inv0)>> /\ *)
+(*                    <<MEM_UNARY: InvMem.Unary.sem conf gmax public st1.(Mem) invmem0>>. *)
+(* Proof. *)
+(*   destruct mem_change; *)
+(*     try by (destruct cmd; ss; des; congruence). *)
+(*   - splits. *)
+(*     admit. *)
+(*     admit. *)
+    
+    
+(*     (* + econs. *) *)
+(*     (*   { ii. ss. unfold ForgetMemory.unary in *. *) *)
+(*     (*     exploit forget_memory_def_sep_mem; eauto. i. *) *)
+(*     (*     exploit sem_expr_equiv_except_mem; eauto. *) *)
+(*     (*     { instantiate (1:= (fst x)). *) *)
+(*     (*       des; try by left; eauto. *) *)
+(*     (*       right. unfold ForgetMemory.is_noalias_ExprPair in *. des_bool. des. ss. *) *)
+(*     (*     } *) *)
+(*     (*     exploit sem_expr_equiv_except_mem; eauto. *) *)
+(*     (*     { instantiate (1:= (snd x)). *) *)
+(*     (*       des; try by left; eauto. *) *)
+(*     (*       right. unfold ForgetMemory.is_noalias_ExprPair in *. des_bool. des. ss. *) *)
+(*     (*     } *) *)
+(*     (*     i. *) *)
+(*     (*     inv STATE. *) *)
+(*     (*     exploit LESSDEF. *) *)
+(*     (*     { des_ifs; eauto. *) *)
+(*     (*       ss. eapply ExprPairSetFacts.filter_iff in H; eauto; try by solve_compat_bool. inv H; eauto. *) *)
+(*     (*     } *) *)
+(*     (*     { rewrite x0. eauto. } *) *)
+(*     (*     i. rewrite <- x2. eauto. *) *)
+(*     (*   } *) *)
+(*     (*   { admit. (* alias *) } *) *)
+(*     (*   { admit. } *) *)
+(*     (*   { admit. } *) *)
+(*     (* + inv MEM_EQUIV. *) *)
+(*     (*   inv MEM_CHANGE_EQUIV. *) *)
+(*     (*   inv MEM. *) *)
+(*     (*   econs; eauto. *) *)
+(*     (*   { i. exploit PRIVATE; eauto. i. des. *) *)
+(*     (*     split; eauto. *) *)
+(*     (*     admit. (* nextblock preserved after mstore *) } *) *)
+(*     (*   { i. exploit PRIVATE_PARENT; eauto. i. des. *) *)
+(*     (*     split; eauto. *) *)
+(*     (*     admit. (* same *) } *) *)
+(*     (*   { unfold mem_change_no_private_parent in *. *) *)
+(*     (*     i. exploit MEM_PARENT; eauto. *) *)
+(*     (*     i. rewrite x. *) *)
+(*     (*     (* STORE: (Mem st1) = mstore (Mem st0) ptr .. *) *) *)
+(*     (*     (* mstore says GV2ptr ptr = Some Vptr .. *) *) *)
+(*     (*     (* NO_PRIVATE_PARENT tells us ~In b_ptr (private_parent) *) *) *)
+(*     (*     (* since b is In private_parent, mload_aux ?mem b should be preserved *) *) *)
+(*     (*     admit. *) *)
+(*     (*   } *) *)
+  
+(*   - admit. (* free case - almost same as above *) *)
+(* Admitted. *)
+
+(* Lemma forget_memory_unary_sound_without_def_memory *)
+(*       conf st0 st1 mem_change *)
+(*       cmd invst0 invmem0 inv0 gmax public *)
+(*       (STATE: InvState.Unary.sem conf st0 invst0 invmem0 inv0) *)
+(*       (DEF_MEM: Cmd.get_def_memory cmd = None) *)
+(*       (MEM: InvMem.Unary.sem conf gmax public st0.(Mem) invmem0) *)
+(*       (MEM_EQUIV : state_equiv_except_mem conf st0 st1 mem_change) *)
+(*       (MEM_CHANGE : mem_change_cmd_after conf st0 mem_change cmd inv0) *)
+(*       (NO_PRIVATE_PARENT: mem_change_no_private_parent conf mem_change invmem0.(InvMem.Unary.private_parent)) *)
+(*       (UNIQUE_PRSV: unique_preserved_mem conf st1 inv0) *)
+(*   : <<STATE_UNARY: InvState.Unary.sem conf st1 invst0 invmem0 inv0>> /\ *)
+(*     <<MEM_UNARY: InvMem.Unary.sem conf gmax public st1.(Mem) invmem0>>. *)
+(* Proof. *)
+(*   destruct mem_change. *)
+(*   - destruct cmd; ss. *)
+(*     admit. (* TODO: for alloca *) *)
+(*   - destruct cmd; ss; des; congruence. *)
+(*   - destruct cmd; ss; des; congruence. *)
+(*   - inv MEM_EQUIV. inv STATES_MEM_CHANGE. *)
+(*     rewrite <- MEM_EQ. *)
+(*     esplits; eauto. *)
+(*     eapply unary_sem_eq_locals_mem; try (symmetry in LOCALS_EQ; exact LOCALS_EQ); eauto. *)
+(* Admitted. *)
+
+(* Lemma forget_memory_maydiff_preserved *)
+(*       conf_src st0_src st1_src mem_change_src def_mem_src *)
+(*       conf_tgt st0_tgt st1_tgt mem_change_tgt def_mem_tgt *)
+(*       invst0 invmem0 inv0 *)
+(*       (MEM_EQUIV_SRC : state_equiv_except_mem conf_src st0_src st1_src mem_change_src) *)
+(*       (MEM_EQUIV_TGT : state_equiv_except_mem conf_tgt st0_tgt st1_tgt mem_change_tgt) *)
+(*       (MAYDIFF : forall id : Tag.t * id, *)
+(*           IdTSet.mem id (Invariant.maydiff inv0) = false -> *)
+(*           InvState.Rel.sem_inject st0_src st0_tgt invst0 (InvMem.Rel.inject invmem0) id) *)
+(*   : <<RES: forall id : Tag.t * id, *)
+(*       IdTSet.mem id (Invariant.maydiff (ForgetMemory.t def_mem_src def_mem_tgt inv0)) = false -> *)
+(*       InvState.Rel.sem_inject st1_src st1_tgt invst0 (InvMem.Rel.inject invmem0) id>>. *)
+(* Proof. *)
+(*   ii. *)
+(*   assert (DROP_FORGET_MEMORY:IdTSet.mem id0 (Invariant.maydiff inv0) = false). *)
+(*   { destruct def_mem_src; destruct def_mem_tgt; ss. } *)
+(*   exploit MAYDIFF; eauto. *)
+(*   { inv MEM_EQUIV_SRC. *)
+(*     unfold InvState.Unary.sem_idT in *. *)
+(*     destruct id0 as [[] x]; eauto. *)
+(*     ss. rewrite LOCALS_EQ. eauto. *)
+(*   } *)
+(*   i. des. *)
+(*   esplits; eauto. *)
+(*   inv MEM_EQUIV_TGT. *)
+(*   unfold InvState.Unary.sem_idT in *. *)
+(*   destruct id0 as [[] x]; eauto. *)
+(*   ss. rewrite <- LOCALS_EQ. eauto. *)
+(* Qed. *)
+
+(* Lemma some_injective A (a b:A): *)
+(*   Some a = Some b -> a = b. *)
+(* Proof. *)
+(*   congruence. *)
+(* Qed. *)
+
+(* (* Lemma mem_inject_change *) *)
+(* (*       conf_src st0_src st1_src cmd_src mem_change_src *) *)
+(* (*       conf_tgt st0_tgt st1_tgt cmd_tgt mem_change_tgt *) *)
+(* (*       invmem0 *) *)
+(* (*       (mem_change_of_cmd conf_src st0_src cmd_src = Some mem_change_src) *) *)
+(* (*       () *) *)
+(* (*       (MEM_CHANGE_EQUIV_SRC : states_mem_change conf_src st0_src st1_src mem_change_src) *) *)
+(* (*       (MEM_CHANGE_EQUIV_TGT : states_mem_change conf_tgt st0_tgt st1_tgt mem_change_tgt) *) *)
+(* (*       (MEM_CHANGE_INJECT : mem_change_inject conf_src conf_tgt invmem0 mem_change_src mem_change_tgt) *) *)
+(* (*       (INJECT : memory_sim.MoreMem.mem_inj (InvMem.Rel.inject invmem0) (Mem st0_src) (Mem st0_tgt)) *) *)
+(* (*   : exists invmem1, *) *)
+(* (*     <<ALLOC_INJECT: alloc_inject conf_src conf_tgt st1_src st1_tgt cmd_src cmd_tgt invmem1>> /\ *) *)
+(* (*     <<MEM_INJ: memory_sim.MoreMem.mem_inj (InvMem.Rel.inject invmem1) (Mem st1_src) (Mem st1_tgt)>>. *) *)
+(* (* Proof. *) *)
+(* (* Admitted. *) *)
+
+(* (*   inv MEM_CHANGE_INJECT. *) *)
+(* (*   - inv INJECT. inv MEM_CHANGE_EQUIV_SRC. inv MEM_CHANGE_EQUIV_TGT. *) *)
+(* (*     unfold malloc in *. *) *)
+(* (*     apply some_injective in MALLOC. *) *)
+(* (*     apply some_injective in MALLOC0. *) *)
+(* (*     econs. *) *)
+(* (*     + eapply Memory.Mem.alloc_right_inj; eauto. *) *)
+(* (*       eapply Memory.Mem.alloc_left_unmapped_inj; eauto. *) *)
+(* (*       apply mi_freeblocks. *) *)
+(* (*       eapply Memory.Mem.fresh_block_alloc; eauto. *) *)
+(* (*     + i. apply mi_freeblocks. ii. *) *)
+(* (*       exploit Memory.Mem.valid_block_alloc; try (symmetry; exact MALLOC); eauto. *) *)
+(* (*     + ii. exploit mi_mappedblocks; eauto. i. *) *)
+(* (*       eapply Memory.Mem.valid_block_alloc; eauto. *) *)
+(* (*     + ii. exploit mi_no_overlap; eauto. *) *)
+(* (*       * eapply Memory.Mem.perm_alloc_4; try (symmetry; exact MALLOC); eauto. *) *)
+(* (*         ii. subst. *) *)
+(* (*         hexploit Memory.Mem.fresh_block_alloc; try (symmetry; exact MALLOC); eauto. i. *) *)
+(* (*         exploit mi_freeblocks; eauto. i. clarify. *) *)
+(* (*       * eapply Memory.Mem.perm_alloc_4; try (symmetry; exact MALLOC); eauto. *) *)
+(* (*         ii. subst. *) *)
+(* (*         hexploit Memory.Mem.fresh_block_alloc; try (symmetry; exact MALLOC); eauto. i. *) *)
+(* (*         exploit mi_freeblocks; eauto. i. clarify. *) *)
+(* (*     + ii. exploit mi_representable; eauto. des. *) *)
+(* (*       * left. *) *)
+(* (*         eapply Memory.Mem.perm_alloc_4; try (symmetry; exact MALLOC); eauto. *) *)
+(* (*         ii. subst. *) *)
+(* (*         hexploit Memory.Mem.fresh_block_alloc; try (symmetry; exact MALLOC); eauto. i. *) *)
+(* (*         exploit mi_freeblocks; eauto. i. clarify. *) *)
+(* (*       * right. *) *)
+(* (*         eapply Memory.Mem.perm_alloc_4; try (symmetry; exact MALLOC); eauto. *) *)
+(* (*         ii. subst. *) *)
+(* (*         hexploit Memory.Mem.fresh_block_alloc; try (symmetry; exact MALLOC); eauto. i. *) *)
+(* (*         exploit mi_freeblocks; eauto. i. clarify. *) *)
+(* (*   - inv INJECT. inv MEM_CHANGE_EQUIV_SRC. inv MEM_CHANGE_EQUIV_TGT. *) *)
+(* (*     rewrite <- MEM_EQ; clear MEM_EQ. *) *)
+(* (*     unfold malloc in *. *) *)
+(* (*     apply some_injective in MALLOC. *) *)
+(* (*     econs. *) *)
+(* (*     + eapply Memory.Mem.alloc_left_unmapped_inj; eauto. *) *)
+(* (*       apply mi_freeblocks. *) *)
+(* (*       eapply Memory.Mem.fresh_block_alloc; eauto. *) *)
+(* (*     + i. apply mi_freeblocks. ii. *) *)
+(* (*       exploit Memory.Mem.valid_block_alloc; try (symmetry; exact MALLOC); eauto. *) *)
+(* (*     + ii. exploit mi_mappedblocks; eauto. *) *)
+(* (*     + ii. exploit mi_no_overlap; eauto. *) *)
+(* (*       * eapply Memory.Mem.perm_alloc_4; try (symmetry; exact MALLOC); eauto. *) *)
+(* (*         ii. subst. *) *)
+(* (*         hexploit Memory.Mem.fresh_block_alloc; try (symmetry; exact MALLOC); eauto. i. *) *)
+(* (*         exploit mi_freeblocks; eauto. i. clarify. *) *)
+(* (*       * eapply Memory.Mem.perm_alloc_4; try (symmetry; exact MALLOC); eauto. *) *)
+(* (*         ii. subst. *) *)
+(* (*         hexploit Memory.Mem.fresh_block_alloc; try (symmetry; exact MALLOC); eauto. i. *) *)
+(* (*         exploit mi_freeblocks; eauto. i. clarify. *) *)
+(* (*     + ii. exploit mi_representable; eauto. des. *) *)
+(* (*       * left. *) *)
+(* (*         eapply Memory.Mem.perm_alloc_4; try (symmetry; exact MALLOC); eauto. *) *)
+(* (*         ii. subst. *) *)
+(* (*         hexploit Memory.Mem.fresh_block_alloc; try (symmetry; exact MALLOC); eauto. i. *) *)
+(* (*         exploit mi_freeblocks; eauto. i. clarify. *) *)
+(* (*       * right. *) *)
+(* (*         eapply Memory.Mem.perm_alloc_4; try (symmetry; exact MALLOC); eauto. *) *)
+(* (*         ii. subst. *) *)
+(* (*         hexploit Memory.Mem.fresh_block_alloc; try (symmetry; exact MALLOC); eauto. i. *) *)
+(* (*         exploit mi_freeblocks; eauto. i. clarify. *) *)
+(* (*   - inv INJECT. inv MEM_CHANGE_EQUIV_SRC. inv MEM_CHANGE_EQUIV_TGT. *) *)
+(* (*     rewrite <- MEM_EQ; clear MEM_EQ. *) *)
+(* (*     unfold malloc in *. *) *)
+(* (*     apply some_injective in MALLOC. *) *)
+(* (*     econs. *) *)
+(* (*     + eapply Memory.Mem.alloc_right_inj; eauto. *) *)
+(* (*     + i. apply mi_freeblocks. eauto. *) *)
+(* (*     + ii. exploit mi_mappedblocks; eauto. i. *) *)
+(* (*       eapply Memory.Mem.valid_block_alloc; eauto. *) *)
+(* (*     + ii. exploit mi_no_overlap; eauto. *) *)
+(* (*     + ii. exploit mi_representable; eauto. *) *)
+(* (*   - inv MEM_CHANGE_EQUIV_SRC. inv MEM_CHANGE_EQUIV_TGT. *) *)
+(* (*     unfold mstore in *. des_ifs. *) *)
+(* (*     (* exploit genericvalues_inject.mem_inj_mstore_aux; eauto. *) *) *)
+    
+(* (*     (* Memory.Mem.mem_inj *) *) *)
+(* (*     (*   memory_sim.MoreMem.mem_inj *) *) *)
+(* (*     admit. (* store - store *) *) *)
+(* (*   - inv MEM_CHANGE_EQUIV_SRC. inv MEM_CHANGE_EQUIV_TGT. *) *)
+(* (*     unfold mstore in *. des_ifs. *) *)
+(* (*     admit. (* store to private *) *) *)
+
+(* (*   - inv MEM_CHANGE_EQUIV_SRC. inv MEM_CHANGE_EQUIV_TGT. *) *)
+(* (*     unfold free in *. des_ifs. *) *)
+(* (*     eapply Memory.Mem.free_left_inject; eauto. *) *)
+(* (*     eapply Memory.Mem.free_right_inject; eauto. *) *)
+(* (*     admit. (* free - free *) *) *)
+(* (*   - inv MEM_CHANGE_EQUIV_SRC. inv MEM_CHANGE_EQUIV_TGT. *) *)
+(* (*     eauto. *) *)
+(* (* Admitted. *) *)
+
+  
+
+(*   exploit inject_mem_change; try exact INJECT_EVENT; eauto. intro MC_INJECT. *)
+
+(*   Lemma mem_change_inject_invmem *)
+(*         (MEM : InvMem.Rel.sem conf_src conf_tgt (Mem st0_src) (Mem st0_tgt) invmem0) *)
+(*         (MC_INJECT: mem_change_inject conf_src conf_tgt invmem0 mc_src mc_tgt) *)
+(*         (STATES_MC_SRC: states_mem_change conf_src mem0 mem1 mc_src) *)
+(*         (STATES_MC_TGT: states_mem_change conf_tgt mem0 mem1 mc_tgt) *)
+
+(*         (STATE_EQUIV_SRC : state_equiv_except_mem conf_src {| EC := EC st1_src; ECS := ECS st1_src; Mem := Mem st0_src |} st1_src mc) *)
+(*         (STATE_EQUIV_TGT : state_equiv_except_mem conf_tgt {| EC := EC st1_tgt; ECS := ECS st1_tgt; Mem := Mem st0_tgt |} st1_tgt mc) *)
+(*     : exists invmem1, *)
+(*       <<ALLOC_INJECT: alloc_inject conf_src conf_tgt st1_src st1_tgt cmd_src cmd_tgt invmem1>> /\ *)
+(*       <<MEM_INJ: memory_sim.MoreMem.mem_inj (InvMem.Rel.inject invmem1) (Mem st1_src) (Mem st1_tgt)>>.         *)
+  
+    
+                                          
+(*         mem_change_cmd_after *)
+
+
+(*         (* Lemma step_equiv_except_mem *) *)
+(* (*       conf st0 st1 evt *) *)
+(* (*       cmd cmds *) *)
+(* (*       invst0 invmem0 inv0 inv1 *) *)
+(* (*       public gmax *) *)
+(* (*       (STATE: InvState.Unary.sem conf st0 invst0 invmem0 inv0) *) *)
+(* (*       (MEM: InvMem.Unary.sem conf gmax public st0.(Mem) invmem0) *) *)
+(* (*       (NONCALL: Instruction.isCallInst cmd = false) *) *)
+(* (*       (CMDS: CurCmds st0.(EC) = cmd :: cmds) *) *)
+(* (*       (FORGET: inv_unary_forgot inv1 (AtomSetImpl_from_list (option_to_list (Cmd.get_def cmd)))) *) *)
+(* (*       (STEP: sInsn conf st0 st1 evt) *) *)
+(* (*   : exists mc, *) *)
+(* (*     <<MEM_CH_REL: mem_change_cmd conf st0 mc cmd>> /\ *) *)
+(* (*     <<STATE_EQUIV: state_equiv_except_mem conf (mkState st1.(EC) st1.(ECS) st0.(Mem)) st1 mc>>. *) *)
+(* (* Proof. *) *)
+(* (*   inv STEP; destruct cmd; inv CMDS; ss; *) *)
+(* (*     try by esplits; eauto; econs; eauto; econs; eauto. *) *)
+(* (*   - admit. (* malloc , should know newly allocated block is unique *) *) *)
+(* (*   - admit. (* alloca *) *) *)
+(* (* Admitted. *) *)
+
+(* (* Lemma step_unique_preserved_mem *) *)
+(* (*       conf st0 st1 evt *) *)
+(* (*       cmd cmds inv0 *) *)
+(* (*       (STATE: AtomSetImpl.For_all (InvState.Unary.sem_unique conf (mkState st1.(EC) st1.(ECS) st0.(Mem))) *) *)
+(* (*                                   inv0.(Invariant.unique)) *) *)
+(* (*       (NONCALL: Instruction.isCallInst cmd = false) *) *)
+(* (*       (CMDS: CurCmds st0.(EC) = cmd :: cmds) *) *)
+(* (*       (STEP: sInsn conf st0 st1 evt) *) *)
+(* (*       (UNIQUE_NOT_LEAKED: forall x (MEM:AtomSetImpl.mem x inv0.(Invariant.unique) = true), *) *)
+(* (*                                  AtomSetImpl.mem x (AtomSetImpl_from_list (Cmd.get_leaked_ids cmd)) = false) *) *)
+(* (*   : unique_preserved_mem conf st1 inv0. *) *)
+(* (* Proof. *) *)
+(* (*   inv STEP; ss; *) *)
+(* (*     try (inv CMDS; ss; *) *)
+(* (*          ii; specialize_unique; eauto). *) *)
+(* (*   { admit. (* load malloc -> undef *) } *) *)
+(* (*   { admit. (* load after free: use Memory.Mem.load_free_2 maybe *) } *) *)
+(* (*   { admit. (* load alloca *) } *) *)
+(* (*   { admit. (* load after store *) } *) *)
+(* (* Admitted. *) *)
+
+(* (* Lemma mem_change_cmd_state_transition *) *)
+(* (*       conf st0 st1 evt cmd cmds mc inv0 *) *)
+(* (*       (CMD: CurCmds (EC st0) = cmd :: cmds) *) *)
+(* (*       (NONCALL: Instruction.isCallInst cmd = false) *) *)
+(* (*       (STEP: sInsn conf st0 st1 evt) *) *)
+(* (*       (MEM_CH_REL: mem_change_cmd conf st0 mc cmd) *) *)
+(* (*       (FORGET: inv_unary_forgot inv0 (AtomSetImpl_from_list (option_to_list (Cmd.get_def cmd)))) *) *)
+(* (*   : mem_change_cmd_after conf {| EC := EC st1; ECS := ECS st1; Mem := Mem st0 |} mc cmd inv0. *) *)
+(* (* Proof. *) *)
+(* (*   destruct cmd; ss; *) *)
+(* (*     inv STEP; ss; *) *)
+(* (*       des; esplits; eauto. *) *)
+(* (*   admit. (* easy *) *) *)
+(* (* Admitted. *) *)
+
+
+  
+(* Admitted. *)
+
+(* (* Lemma forget_memory_sound *) *)
+(* (*       m_src conf_src st0_src st1_src mem_change_src cmd_src *) *)
+(* (*       m_tgt conf_tgt st0_tgt st1_tgt mem_change_tgt cmd_tgt *) *)
+(* (*       invst0 invmem0 inv0 *) *)
+(* (*       (CONF: InvState.valid_conf m_src m_tgt conf_src conf_tgt) *) *)
+(* (*       (STATE: InvState.Rel.sem conf_src conf_tgt st0_src st0_tgt invst0 invmem0 inv0) *) *)
+(* (*       (MEM: InvMem.Rel.sem conf_src conf_tgt st0_src.(Mem) st0_tgt.(Mem) invmem0) *) *)
+(* (*       (MEM_EQUIV_SRC: state_equiv_except_mem *) *)
+(* (*                         conf_src *) *)
+(* (*                         st0_src st1_src *) *)
+(* (*                         mem_change_src) *) *)
+(* (*       (MEM_EQUIV_TGT: state_equiv_except_mem *) *)
+(* (*                         conf_tgt *) *)
+(* (*                         st0_tgt st1_tgt *) *)
+(* (*                         mem_change_tgt) *) *)
+(* (*       (MEM_CHANGE_SRC: mem_change_cmd_after conf_src st0_src mem_change_src cmd_src inv0.(Invariant.src)) *) *)
+(* (*       (MEM_CHANGE_TGT: mem_change_cmd_after conf_tgt st0_tgt mem_change_tgt cmd_tgt inv0.(Invariant.tgt)) *) *)
+(* (*       (MEM_CHANGE_INJECT: mem_change_inject conf_src conf_tgt invmem0 mem_change_src mem_change_tgt) *) *)
+(* (*       (UNIQUE_PRSV_SRC: unique_preserved_mem conf_src st1_src inv0.(Invariant.src)) *) *)
+(* (*       (UNIQUE_PRSV_TGT: unique_preserved_mem conf_tgt st1_tgt inv0.(Invariant.tgt)) *) *)
+(* (*   : *) *)
+(* (*     exists invmem1, *) *)
+(* (*       <<ALLOC_INJECT: alloc_inject conf_src conf_tgt st1_src st1_tgt cmd_src cmd_tgt invmem1>> /\ *) *)
+(* (*       <<STATE: InvState.Rel.sem conf_src conf_tgt st1_src st1_tgt invst0 invmem1 *) *)
+(* (*                                 (ForgetMemory.t (Cmd.get_def_memory cmd_src) (Cmd.get_def_memory cmd_tgt) inv0) >> /\ *) *)
+(* (*       <<MEM: InvMem.Rel.sem conf_src conf_tgt st1_src.(Mem) st1_tgt.(Mem) invmem1>> /\ *) *)
+(* (*       <<MEMLE: InvMem.Rel.le invmem0 invmem1>>. *) *)
+(* (* Proof. *) *)
+(* (*   exploit mem_change_inject_no_private_parent_src; eauto. intro NO_PRIVATE_PARENT_SRC. *) *)
+(* (*   exploit mem_change_inject_no_private_parent_tgt; eauto. intro NO_PRIVATE_PARENT_TGT. *) *)
+(* (*   inv STATE. inv MEM. *) *)
+
+(* (*   destruct (Cmd.get_def_memory cmd_src) eqn:DEF_MEM_SRC; *) *)
+(* (*     destruct (Cmd.get_def_memory cmd_tgt) eqn:DEF_MEM_TGT. *) *)
+(* (*   - hexploit forget_memory_unary_sound_with_def_memory; try exact SRC; try exact DEF_MEM_SRC; eauto. i. des. *) *)
+(* (*     hexploit forget_memory_unary_sound_with_def_memory; try exact TGT; try exact DEF_MEM_TGT; eauto. i. des. *) *)
+(* (*     hexploit forget_memory_maydiff_preserved; try exact MAYDIFF; eauto. i. des. *) *)
+(* (*     inv MEM_EQUIV_SRC. inv MEM_EQUIV_TGT. *) *)
+(* (*     hexploit mem_inject_change; try exact MEM_CHANGE_INJECT; eauto. i. *) *)
+(* (*     esplits; econs; eauto. *) *)
+(* (*   - hexploit forget_memory_unary_sound_with_def_memory; try exact SRC; try exact DEF_MEM_SRC; eauto. i. des. *) *)
+(* (*     hexploit forget_memory_unary_sound_without_def_memory; try exact TGT; try exact DEF_MEM_TGT; eauto. i. des. *) *)
+(* (*     hexploit forget_memory_maydiff_preserved; try exact MAYDIFF; eauto. i. des. *) *)
+(* (*     inv MEM_EQUIV_SRC. inv MEM_EQUIV_TGT. *) *)
+(* (*     hexploit mem_inject_change; try exact MEM_CHANGE_INJECT; eauto. i. *) *)
+(* (*     esplits; econs; eauto. *) *)
+(* (*   - hexploit forget_memory_unary_sound_without_def_memory; try exact SRC; try exact DEF_MEM_SRC; eauto. i. des. *) *)
+(* (*     hexploit forget_memory_unary_sound_with_def_memory; try exact TGT; try exact DEF_MEM_TGT; eauto. i. des. *) *)
+(* (*     hexploit forget_memory_maydiff_preserved; try exact MAYDIFF; eauto. i. des. *) *)
+(* (*     inv MEM_EQUIV_SRC. inv MEM_EQUIV_TGT. *) *)
+(* (*     hexploit mem_inject_change; try exact MEM_CHANGE_INJECT; eauto. i. *) *)
+(* (*     esplits; econs; eauto. *) *)
+(* (*   - hexploit forget_memory_unary_sound_without_def_memory; try exact SRC; try exact DEF_MEM_SRC; eauto. i. des. *) *)
+(* (*     hexploit forget_memory_unary_sound_without_def_memory; try exact TGT; try exact DEF_MEM_TGT; eauto. i. des. *) *)
+(* (*     hexploit forget_memory_maydiff_preserved; try exact MAYDIFF; eauto. i. des. *) *)
+(* (*     inv MEM_EQUIV_SRC. inv MEM_EQUIV_TGT. *) *)
+(* (*     hexploit mem_inject_change; try exact MEM_CHANGE_INJECT; eauto. i. *) *)
+(* (*     esplits; econs; eauto. *) *)
+(* (* Qed. *) *)
